theories/coneris/examples/lazy_rand/lazy_rand_race.v
@@ -1,0 +1,156 @@
+From iris.algebra Require Import excl_auth.
+From clutch.coneris Require Import coneris par spawn lazy_rand_interface.
+  
+Set Default Proof Using "Type*".
+Section lemmas.
+  Context `{!inG Σ (excl_authR boolO)}.
+
+  (* Helpful lemmas *)
+  Lemma ghost_var_alloc b :
+    ⊢ |==> ∃ γ, own γ (●E b) ∗ own γ (◯E b).
+  Proof.
+    iMod (own_alloc (●E b ⋅ ◯E b)) as (γ) "[??]".
+    - by apply excl_auth_valid.
+    - by eauto with iFrame.
+  Qed.
+
+  Lemma ghost_var_agree γ b c :
+    own γ (●E b) -∗ own γ (◯E c) -∗ ⌜ b = c ⌝.
+  Proof.
+    iIntros "Hγ● Hγ◯".
+    by iCombine "Hγ● Hγ◯" gives %->%excl_auth_agree_L.
+  Qed.
+
+  Lemma ghost_var_update γ b' b c :
+    own γ (●E b) -∗ own γ (◯E c) ==∗ own γ (●E b') ∗ own γ (◯E b').
+  Proof.
+    iIntros "Hγ● Hγ◯".
+    iMod (own_update_2 _ _ _ (●E b' ⋅ ◯E b') with "Hγ● Hγ◯") as "[$$]".
+    { by apply excl_auth_update. }
+    done.
+  Qed.
+End lemmas.
+
+
+Section race.
+  Context `{!conerisGS Σ, !spawnG Σ, c:!lazy_rand 1, !inG Σ (excl_authR boolO) }.
+
+  
+  Definition race_prog : expr :=
+  let: "r" := init_lazy_rand #() in
+  ( lazy_read_rand "r" (allocate_tape #()) #0)
+  |||
+  ( lazy_read_rand "r" (allocate_tape #()) #1).
+
+  Lemma race_prog_spec:
+  {{{ ↯ (1/2) }}}
+    race_prog
+    {{{ (n:nat), RET ((#n,#n),(#n,#n))%Z; ⌜n<=1⌝ }}}.
+  Proof.
+    iIntros (Φ) "Herr HΦ".
+    rewrite /race_prog.
+    iMod (ghost_var_alloc false) as (γ) "[Hauth Hfrag]".
+    wp_apply (lazy_rand_init (nroot.@"1") (λ x,  ⌜x = None⌝ ∗ own γ (◯E false) ∨
+                                                ∃ x1, ⌜x=Some (x1, x1)⌝ ∗ (own γ (◯E true)))%I
+                                                
+               with "[Hfrag]").
+    { iLeft. iFrame. done. }
+    iIntros (?) "(%&%&%&#Hinv)".
+    iMod (inv_alloc (nroot.@"inv") _ (own γ (●E false) ∗ ↯ (1/2)∨ own γ (●E true))%I with "[Herr Hauth ]") as "#Hinv2".
+    { iLeft. iFrame. }
+    wp_pures.
+    wp_apply (wp_par (λ res, ∃ (n:nat), ⌜(#n, #n)%V = res⌝ ∗ rand_frag n n _)%I
+                (λ res, ∃ (n:nat), ⌜(#n, #n)%V = res⌝ ∗ rand_frag n n _)%I with "[][]").
+    - wp_apply (lazy_rand_alloc_tape _ _ ).
+      { iSplit; last by iIntros. done. }
+      iIntros (α) "[Ht _]".
+      replace #0 with (# (Z.of_nat 0)) by done.
+      wp_apply (lazy_rand_spec _ _ _ _ _ _ (λ x y, ⌜x=y⌝ ∗ rand_frag x x _)%I (λ x y, ⌜x=y⌝ ∗ rand_frag x x _)%I with "[-]").
+      + iSplit; first done.
+        simpl. iIntros (n m) "H1 Hauth Htauth".
+        iApply (state_update_inv_acc with "Hinv2").
+        { apply subseteq_difference_r; last done.
+          by apply ndot_preserve_disjoint_r, ndot_ne_disjoint.
+        }
+        iIntros ">[[H2 Herr]|H2]"; iDestruct "H1" as "[(->&?)|(%&->&?)]"; iDestruct (ghost_var_agree with "[$][$]") as "%"; simplify_eq.
+        * iMod (rand_tape_presample _ _ _ _ _ _ _ _ _ _ (λ x, if bool_decide (fin_to_nat x = 0%nat) then 0 else 1) with "[$][$][$][$]") as "(%n&?&?&?)".
+          { apply subseteq_difference_r.
+            - by apply ndot_preserve_disjoint_l, ndot_ne_disjoint.
+            - apply subseteq_difference_r; last done.
+              by apply ndot_ne_disjoint.
+          }
+          { intros. case_bool_decide; simpl; lra. }
+          { rewrite SeriesC_finite_foldr/=. lra. }
+          iAssert (⌜fin_to_nat n=0%nat⌝)%I as "%Heq".
+          { case_bool_decide; first done. iDestruct (ec_contradict with "[$]") as "[]".
+            simpl. lra. }
+          rewrite bool_decide_eq_true_2; last done.
+          iFrame.
+          iMod (ghost_var_update with "[$][$]") as "[H1 H2]".
+          iFrame.
+          iModIntro.
+          iIntros. iSplitR "H1"; last first.
+          { by iRight. }
+          iMod (rand_auth_update (0,_) with "[$]") as "?".
+          { simpl. lia. }
+          iDestruct (rand_auth_duplicate with "[$]") as "#?".
+          rewrite Heq. iFrame. iIntros. 
+          iModIntro. simpl. repeat iSplit; try done.
+          iRight. iFrame. iExists _. done. 
+        * iDestruct (rand_auth_duplicate with "[$]") as "#?".
+          iFrame. iModIntro.
+          repeat iSplit; try done.
+          iRight. iFrame. by iExists _.
+      + by iIntros (??) "[(->&#$)|(->&#$)]".
+    - wp_apply (lazy_rand_alloc_tape _ _ ).
+      { iSplit; last by iIntros. done. }
+      iIntros (α) "[Ht _]".
+      replace #1 with (# (Z.of_nat 1)) by done.
+      wp_apply (lazy_rand_spec _ _ _ _ _ _ (λ x y, ⌜x=y⌝ ∗ rand_frag x x _)%I (λ x y, ⌜x=y⌝ ∗ rand_frag x x _)%I with "[-]").
+      + iSplit; first done.
+        simpl. iIntros (n m) "H1 Hauth Htauth".
+        iApply (state_update_inv_acc with "Hinv2").
+        { apply subseteq_difference_r; last done.
+          by apply ndot_preserve_disjoint_r, ndot_ne_disjoint.
+        }
+        iIntros ">[[H2 Herr]|H2]"; iDestruct "H1" as "[(->&?)|(%&->&?)]"; iDestruct (ghost_var_agree with "[$][$]") as "%"; simplify_eq.
+        * iMod (rand_tape_presample _ _ _ _ _ _ _ _ _ _ (λ x, if bool_decide (fin_to_nat x = 1%nat) then 0 else 1) with "[$][$][$][$]") as "(%n&?&?&?)".
+          { apply subseteq_difference_r.
+            - by apply ndot_preserve_disjoint_l, ndot_ne_disjoint.
+            - apply subseteq_difference_r; last done.
+              by apply ndot_ne_disjoint.
+          }
+          { intros. case_bool_decide; simpl; lra. }
+          { rewrite SeriesC_finite_foldr/=. lra. }
+          iAssert (⌜fin_to_nat n=1%nat⌝)%I as "%Heq".
+          { case_bool_decide; first done. iDestruct (ec_contradict with "[$]") as "[]".
+            simpl. lra. }
+          rewrite bool_decide_eq_true_2; last done.
+          iFrame.
+          iMod (ghost_var_update with "[$][$]") as "[H1 H2]".
+          iFrame.
+          iModIntro.
+          iIntros. iSplitR "H1"; last first.
+          { by iRight. }
+          iMod (rand_auth_update (1,_) with "[$]") as "?".
+          { simpl. lia. }
+          iDestruct (rand_auth_duplicate with "[$]") as "#?".
+          rewrite Heq. iFrame. iIntros. 
+          iModIntro. simpl. repeat iSplit; try done.
+          iRight. iFrame. iExists _. done. 
+        * iDestruct (rand_auth_duplicate with "[$]") as "#?".
+          iFrame. iModIntro.
+          repeat iSplit; try done.
+          iRight. iFrame. by iExists _.
+      + by iIntros (??) "[(->&#$)|(->&#$)]". 
+    - iIntros (??) "[(%&<-&?) (%&<-&?)]".
+      iDestruct (rand_frag_frag_agree with "[$][$]") as "[% %]".
+      simplify_eq.
+      iApply "HΦ".
+      iNext.
+      iDestruct (rand_frag_valid with "[$]") as "%".
+      done.
+  Qed.
+      
+  
+End race.
